int working but not ok

AnalysisNotes/Integer/Int.lean
@@ -8,51 +8,79 @@ structure ℤ where
 
 namespace ℤ
 
-instance : Zero ℤ where
-  zero := ⟨0, 0⟩
+def fromNat : Nat → ℤ
+  | 0 => ⟨0, 0⟩
+  | n => ⟨ℕ.fromNat n, 0⟩
 
-instance : One ℤ where
-  one := ⟨1, 0⟩
+instance (n : Nat) : OfNat ℤ n where
+  ofNat := fromNat n
+
+#eval (2 : ℤ)
+
+def toInt : ℤ → Int := λ ⟨a, b⟩ => a.toNat - b.toNat
+
+instance : Repr ℤ where
+  reprPrec n _ := repr (toInt n)
+
+#eval ℤ.mk 0 2
+#eval ℤ.mk 0 0
+#eval ℤ.mk 3 2
 
 @[simp] def neg : ℤ → ℤ := λ ⟨a, b⟩ => ⟨b, a⟩
 
 notation "⁻" x => neg x
 
-#check ⁻1
+#eval ⁻0
 #eval ⁻1
 
-@[simp] theorem zero_eq_neg_zero : (0 : ℤ) = ⁻0 := rfl
+@[simp] def eqv : ℤ → ℤ → Prop := λ ⟨a, b⟩ ⟨c, d⟩ => a + d = b + c
 
+notation x " ∼ " y => eqv x y
 
-@[simp] def eq : ℤ → ℤ → Prop := λ ⟨a, b⟩ ⟨c, d⟩ => a + d = b + c
-
-notation x " ∼ " y => eq x y
-
-@[simp] theorem eq_refl (x : ℤ) : x ∼ x := by simp
-@[simp] theorem eq_symm (x y : ℤ) (h : x ∼ y) : y ∼ x := by simp at *; rw [h]
-@[simp] theorem eq_trans (x y z : ℤ) (h₁ : x ∼ y) (h₂ : y ∼ z) : x ∼ z := by
+@[simp] theorem eqv_refl (x : ℤ) : x ∼ x := by simp
+@[simp] theorem eqv_symm {x y : ℤ} (h : x ∼ y) : y ∼ x := by simp at *; rw [h]
+@[simp] theorem eqv_trans {x y z : ℤ} (h₁ : x ∼ y) (h₂ : y ∼ z) : x ∼ z := by
   simp at *
   apply ℕ.add_cancel_right _ _ y.a
+  -- LHS
   rw [ℕ.add_assoc, ℕ.add_comm z.b, h₂, ← ℕ.add_assoc, ℕ.add_comm x.a]
+  -- RHS
   rw [ℕ.add_assoc z.a x.b, ℕ.add_comm x.b, ← h₁, ← ℕ.add_assoc]
+
+instance : DecidableRel eqv :=
+  λ ⟨a, b⟩ ⟨c, d⟩ => inferInstanceAs (Decidable (a + d = b + c))
+
+#eval 0 ∼ ⁻0
+#eval (1 ∼ ⁻1) -> False
 
 @[simp] def add : ℤ → ℤ → ℤ := λ ⟨a, b⟩ ⟨c, d⟩ => ⟨a + c, b + d⟩
 
 instance : Add ℤ where
   add := add
 
-#check (1 : ℤ) + 1
-#eval (1 : ℤ) + 1
+#eval (2 : ℤ) + 3
+#eval (2 : ℤ) + ⁻3
 
-
-theorem add_inv (x : ℤ) : (x + ⁻x) ∼ 0 := by simp
-
-
-@[simp] def sub : ℤ → ℤ → ℤ := λ a b => a + ⁻b
+@[simp] def sub (x y : ℤ) : ℤ := x + ⁻y
 
 instance : Sub ℤ where
   sub := sub
 
-#eval (1 : ℤ) - 1
+#eval ((1 : ℤ) - 1) ∼ 0
+
+@[simp] def mul : ℤ → ℤ → ℤ := λ ⟨a, b⟩ ⟨c, d⟩ => ⟨a * d, b * c⟩
+
+instance : Mul ℤ where
+  mul := mul
+
+#check (⁻3) * 2
+#eval  (⁻3) * 2
+
+instance intSetoid : Setoid ℤ where
+  r := eqv
+  iseqv := ⟨eqv_refl, eqv_symm, eqv_trans⟩
 
 end ℤ
+
+
+-- def ℤ₁ := Quotient ℤ.intSetoid
